examples/noBasisRed/DiffEvalTest.v
@@ -1,0 +1,990 @@
+Require Import Coq.Lists.List.
+Import ListNotations.
+Require Import Coq.Strings.String.
+Require Import StructTact.StructTactics.
+Require Import Omega.
+Require Import Coq.Logic.Eqdep_dec.
+
+Require Import CakeSem.Utils.
+Require Import FFI.
+Require Import CakeSem.Namespace.
+Require Import CakeSem.CakeAST.
+Require Import CakeSem.SemanticsAux.
+Require Import CakeSem.Evaluate.
+
+Require Import NoBasis.
+
+Definition init_env : sem_env val := empty_sem_env.
+Definition init_store := empty_store val.
+
+Parameter A : Type.
+Parameter init_ffi_st : ffi_state A.
+Definition init_state := Build_state 0 init_store init_ffi_st 0 0.
+
+Definition my_env :=
+  {| sev := [(Short "answer",
+              Conv (Some (TypeStamp "S" 0))
+                   [Conv (Some (TypeStamp "S" 0))
+                         [Conv (Some (TypeStamp "S" 0))
+                               [Conv (Some (TypeStamp "S" 0))
+                                     [Conv (Some (TypeStamp "S" 0)) [Conv (Some (TypeStamp "O" 0)) []]]]]]);
+               (Short "three",
+                Conv (Some (TypeStamp "S" 0))
+                     [Conv (Some (TypeStamp "S" 0))
+                           [Conv (Some (TypeStamp "S" 0)) [Conv (Some (TypeStamp "O" 0)) []]]]);
+               (Short "two",
+                Conv (Some (TypeStamp "S" 0)) [Conv (Some (TypeStamp "S" 0)) [Conv (Some (TypeStamp "O" 0)) []]]);
+               (Short "plus",
+                Recclosure
+                  {| sev := []; sec := [(Short "S", (1, TypeStamp "S" 0)); (Short "O", (0, TypeStamp "O" 0))] |}
+                  [("plus", "x",
+                    EFun "y"
+                         (ELannot
+                            (EMat (ELannot (EVar (Short "x")) [0])
+                                  [(Pcon (Some (Short "O")) [], ELannot (EVar (Short "y")) [0]);
+                                     (Pcon (Some (Short "S")) [Pvar "xp"],
+                                      ELannot
+                                        (ECon (Some (Short "S"))
+                                              [EApp Opapp
+                                                    [ELannot
+                                                       (EApp Opapp
+                                                             [ELannot (EVar (Short "plus")) [0]; ELannot (EVar (Short "xp")) [0]])
+                                                       [0]; ELannot (EVar (Short "y")) [0]]]) [0])]) [0]))] "plus")];
+     sec := [(Short "S", (1, TypeStamp "S" 0)); (Short "O", (0, TypeStamp "O" 0))] |}.
+
+Definition my_st := {| clock := 0; refs := []; ffi := init_ffi_st; next_type_stamp := 1; next_exn_stamp := 0 |}.
+
+
+Inductive namespace_extended (M N V : Type) : namespace M N V -> namespace M N V -> Prop :=
+| Reflexive_ns_extended : forall (ns : namespace M N V), namespace_extended M N V ns ns
+| Extended_by_one : forall (ns0 ns1 : namespace M N V) (p : ident M N * V),
+    namespace_extended M N V ns0 ns1 -> namespace_extended M N V ns0 (p::ns1).
+
+Lemma empty_always_extendable :
+  forall (M N V : Type) (ns : namespace M N V), namespace_extended M N V [] ns.
+Proof.
+  induction ns; constructor; assumption.
+Qed.
+
+Lemma idk :
+  forall (M N V : Type) (ns0 ns1 : namespace M N V) (id : ident M N) (v : V),
+    namespace_extended M N V ns0 ns1 ->
+    namespace_extended M N V ((id,v)::ns0) ((id,v)::ns1).
+Proof.
+  induction ns0.
+  intros ns1 id v H.
+  constructor.
+Abort.
+
+Theorem namespace_extended_dec :
+  forall (M N V : Type)
+    (m_dec : forall (m0 m1 : M), {m0 = m1} + {m0 <> m1})
+    (n_dec : forall (n0 n1 : N), {n0 = n1} + {n0 <> n1})
+    (v_dec : forall (v0 v1 : V), {v0 = v1} + {v0 <> v1})
+    (ns0 ns1 : namespace M N V),
+    {namespace_extended M N V ns0 ns1} + {not (namespace_extended M N V ns0 ns1)}.
+Proof.
+  intros M N V m_dec n_dec v_dec.
+  induction ns0; induction ns1.
+  - left. constructor.
+  - left. apply empty_always_extendable.
+  - right. intro contra. inv contra.
+  - destruct IHns1.
+    + left. constructor. assumption.
+    + destruct (list_eq_dec (pair_eq_dec _ _ (ident_eq_dec _ _ m_dec n_dec) v_dec) ns0 ns1).
+      destruct (pair_eq_dec _ _ (ident_eq_dec _ _ m_dec n_dec) v_dec a a0).
+      subst.
+      left. constructor.
+      right. intro contra.
+      subst.
+      inv contra. congruence.
+      apply n. congruence.
+      right. intro contra.
+      inv contra. congruence.
+      apply n. congruence.
+Qed.
+
+Definition environment_extended (env0 env1 : sem_env val) : Prop :=
+  namespace_extended _ _ _ (sev env0) (sev env1) /\
+  namespace_extended _ _ _ (sec env0) (sec env1).
+
+
+Definition namespace_subset (M N V : Type) (ns0 ns1 : namespace M N V)
+           (m_dec : forall (m0 m1 : M), {m0 = m1} + {m0 <> m1})
+           (n_dec : forall (n0 n1 : N), {n0 = n1} + {n0 <> n1})
+  : Prop :=
+  forall (id : ident M N) (v : V),
+    nsLookup (ident_eq_dec _ _ m_dec n_dec) id ns0 = Some v ->
+    nsLookup (ident_eq_dec _ _ m_dec n_dec) id ns1 = Some v.
+
+Definition env_subset (env0 env1 : sem_env val) : Prop :=
+  namespace_subset _ _ _ (sev env0) (sev env1) string_dec string_dec /\
+  namespace_subset _ _ _ (sec env0) (sec env1) string_dec string_dec.
+
+(* Theorem namespace_subset_dec : *)
+(*   forall (M N V : Type) (ns0 ns1 : namespace M N V) *)
+(*     (m_dec : forall (m0 m1 : M), {m0 = m1} + {m0 <> m1}) *)
+(*     (n_dec : forall (n0 n1 : N), {n0 = n1} + {n0 <> n1}), *)
+(*     {namespace_subset _ _ _ ns0 ns1 m_dec n_dec} + {not (namespace_subset _ _ _ ns0 ns1 m_dec n_dec)}. *)
+(* Proof. *)
+(*   intros M N V ns0 ns1 m_dec n_dec. *)
+(*   generalize dependent ns1. *)
+(*   induction ns0. intros ns1. *)
+(*   - left. unfold namespace_subset. *)
+(*     intros id v H. inv H. *)
+(*   - destruct ns1. *)
+(*     + right. unfold namespace_subset. *)
+(*       intro contra. *)
+(*       unfold nsLookup in contra. simpl in contra. *)
+
+Inductive nat_rel_cake_nat (typestamp : nat) : nat -> val -> Prop :=
+| zero_rel : nat_rel_cake_nat typestamp 0 (Conv (Some (TypeStamp "O" typestamp)) [])
+| suc_rel  : forall (n : nat) (prev : val), nat_rel_cake_nat typestamp n prev -> nat_rel_cake_nat typestamp (S n) (Conv (Some (TypeStamp "S" typestamp)) [prev]).
+
+
+Fixpoint nat_to_cake_nat (typestamp : nat) (n : nat) : val :=
+  match n with
+  | O => (Conv (Some (TypeStamp "O" typestamp)) [])
+  | S n' => (Conv (Some (TypeStamp "S" typestamp)) [nat_to_cake_nat typestamp n'])
+  end.
+
+Lemma nat_to_cake_nat_rel : forall (typestamp n : nat), nat_rel_cake_nat typestamp n (nat_to_cake_nat typestamp n).
+Proof.
+  induction n; simpl; constructor; assumption.
+Qed.
+
+Ltac step_fuel_in fuel H := destruct fuel; simpl in H.
+
+Definition evaluate_diverges {ffi' : Type} (st : state ffi') (env : sem_env val) (e : exp) : Prop :=
+  forall (fuel : nat), exists (st' : state ffi'), evaluate [e] fuel st env = (st', Rerr (Rabort Rtimeout_error)).
+
+Lemma exists_fuel_no_divergence : forall (st : state A) (env : sem_env val) (e : exp) (v : val),
+    (exists (f : nat), evaluate [e] f st env = (st, Rval [v])) -> ~ evaluate_diverges st env e.
+Proof.
+  intros st env e.
+  induction e;
+    intros va H contra;
+    inversion H as [f H']; specialize (contra f); inversion contra as [st' contra']; clear H; clear contra;
+     rewrite H' in contra'; inversion contra'.
+Qed.
+
+Require Import Equations.Equations.
+
+Ltac inv H := inversion H; subst; clear H.
+Lemma Forall''_app : forall (T : Type) (P : T -> Type) (l : list T) (a : T), Forall'' P l -> P a -> Forall'' P (l ++ [a]).
+  intros.
+  induction l.
+  constructor.
+  assumption.
+  assumption.
+  inv X.
+  constructor.
+  assumption.
+  apply IHl.
+  assumption.
+Qed.
+
+Lemma Forall''_rev : forall (T : Type) (P : T -> Type) (l : list T),
+    Forall'' P l -> Forall'' P (rev l).
+  intros.
+  induction l.
+  constructor.
+  inv X.
+  simpl.
+  apply Forall''_app; auto.
+Qed.
+
+Lemma evaluate_sing : forall (e : exp) (f : nat) (st st' : state A) (env : sem_env val) (vs : list val),
+    eval_or_match true [e] f st env uu uu = (st', Rval vs) -> exists (v : val), vs = [v].
+Proof.
+  intros e f.
+  revert e.
+  induction f; induction e; intros.
+  - unfold evaluate in H. simp eval_or_match in H.
+    destruct (do_con_check (sec env) o (Datatypes.length l)).
+    break_let.
+    destruct r.
+    destruct (build_conv (sec env) o (rev l0)); inv H; eauto.
+    inv H.
+    inv H.
+
+ - unfold evaluate in H. simp eval_or_match in H. simp eval_or_match in H.
+   destruct (nsLookup ident_string_dec i (sev env)); inv H; eauto.
+
+ - unfold evaluate in H. simp eval_or_match in H. simp eval_or_match in H.
+   inv H.
+   eauto.
+
+ - unfold evaluate in H. simp eval_or_match in H. simp eval_or_match in H. inv H.
+
+ - unfold evaluate in H. simp eval_or_match in H.
+   induction X.
+   break_let.
+   simp eval_or_match in H.
+   destruct r. apply IHe in Heqp.
+   destruct Heqp.
+   rewrite H0 in *.
+   simp eval_or_match in H.
+   inv H.
+   inv H.
+   break_let.
+   destruct r.
+   apply IHe in Heqp0.
+   destruct Heqp0.
+   rewrite H0 in *. clear H0.
+   destruct x.
+   simpl in *.
+   simp eval_or_match in H.
+   break_if.
+   break_match.
+   apply IHX in H.
+   apply H.
+   inv H.
+   apply p in H.
+   apply H.
+   inv H.
+   inv H.
+
+ - unfold evaluate in H. simp eval_or_match in H.
+
+ - unfold evaluate in H. simp eval_or_match in H.
+    destruct (do_con_check (sec env) o (Datatypes.length l)).
+    break_let.
+    destruct r.
+    destruct (build_conv (sec env) o (rev l0)); inv H; eauto.
+    inv H.
+    inv H.
+
+ - unfold evaluate in H. simp eval_or_match in H.
+   destruct (nsLookup ident_string_dec i (sev env)).
+   inv H. exists v. reflexivity.
+   inv H.
+
+ - unfold evaluate in H. simp eval_or_match in H.
+   inv H. exists (Closure env v e). reflexivity.
+
+ - unfold evaluate in H. simp eval_or_match in H.
+   break_let.
+   apply Forall''_rev in X.
+   induction X.
+   simp eval_or_match in Heqp.
+   inv Heqp.
+   break_if.
+   simpl in H.
+   inv H.
+   simpl in *.
+   inv H.
+   destruct r.
+   break_if.
+   break_match.
+   break_let.
+   apply IHf in H.
+   apply H.
+   inv H.
+   break_match.
+   break_let.
+   break_let.
+   inv H.
+   destruct r.
+   simpl in *.
+   inv H2.
+   exists v. reflexivity.
+   inv H2.
+   inv H.
+   inv H.
+
+ - unfold evaluate in H. simp eval_or_match in H.
+   break_let.
+   destruct r.
+   apply IHe in Heqp.
+   destruct Heqp.
+   rewrite H0 in *.
+   induction X.
+   simp eval_or_match in H.
+   inv H.
+   destruct x0.
+   simp eval_or_match in *.
+   break_if.
+   break_match.
+   apply IHX.
+   apply H.
+   inv H.
+   apply p in H.
+   apply H.
+   inv H.
+   inv H.
+
+ - unfold evaluate in H. simp eval_or_match in H.
+Qed.
+
+Theorem eval_or_match_cons : forall (st : state A) (env : sem_env val) (e : exp) (es : list exp) (f : nat),
+   eval_or_match true (e::es) f st env uu uu =
+     match eval_or_match true [e] f st env uu uu with
+     | (st', Rval vs) =>
+      match eval_or_match true es f st' env uu uu with
+       | (st'', Rval vs') => (st'', Rval (vs++vs'))
+       | err => err
+      end
+     | err => err
+     end.
+Proof.
+  unfold evaluate.
+  intros. revert e st.
+  destruct es; intros; simpl.
+  destruct (eval_or_match true [e] f st env uu uu).
+  destruct r.
+  simp eval_or_match.
+  rewrite app_nil_r.
+  congruence.
+  congruence.
+  simp eval_or_match.
+  destruct (eval_or_match true [e0] f st env uu uu) eqn:eval1.
+  destruct r.
+  apply evaluate_sing in eval1.
+  destruct eval1. rewrite H. simpl.
+  congruence.
+  congruence.
+Qed.
+
+Theorem evaluate_cons : forall (st : state A) (env : sem_env val) (e : exp) (es : list exp) (f : nat),
+   evaluate (e::es) f st env =
+     match evaluate [e] f st env with
+     | (st', Rval vs) =>
+      match evaluate es f st' env with
+       | (st'', Rval vs') => (st'', Rval (vs++vs'))
+       | err => err
+      end
+     | err => err
+     end.
+Proof.
+  unfold evaluate.
+  apply eval_or_match_cons.
+Qed.
+
+Theorem eval_or_match_app : forall (st : state A) env xs ys f,
+   eval_or_match true (xs ++ ys) f st env uu uu =
+     match eval_or_match true xs f st env uu uu with
+     | (st', Rval vs) =>
+       match eval_or_match true ys f st' env uu uu with
+       | (s'', Rval vs') => (s'', Rval (vs++vs'))
+       | err => err
+       end
+     | err => err
+     end.
+Proof.
+  intros. revert ys st.
+  induction xs; intros. simpl.
+  unfold evaluate.
+  simp eval_or_match.
+  destruct (eval_or_match true ys f st env uu uu).
+  destruct r; simpl; congruence.
+  rewrite eval_or_match_cons.
+  simpl.
+  rewrite eval_or_match_cons.
+  destruct (eval_or_match true [a] f st env uu uu).
+  destruct r.
+  rewrite IHxs.
+  destruct (eval_or_match true xs f s env uu uu ).
+  destruct r.
+  destruct (eval_or_match true ys f s0 env uu uu).
+  destruct r.
+  rewrite app_assoc_reverse.
+  congruence.
+  congruence.
+  congruence.
+  congruence.
+Qed.
+
+Theorem evaluate_app : forall (st : state A) env xs ys f,
+   evaluate (xs ++ ys) f st env =
+     match evaluate xs f st env with
+     | (st', Rval vs) =>
+       match evaluate ys f st' env with
+       | (s'', Rval vs') => (s'', Rval (vs++vs'))
+       | err => err
+       end
+     | err => err
+     end.
+Proof.
+  unfold evaluate; apply eval_or_match_app.
+Qed.
+
+(* Lemma eval_or_match_sing : forall fuel e env (st : state A), *)
+(*   eval_or_match true [e] fuel st env uu uu = *)
+(*   match e with *)
+(*   | EVar n => match nsLookup ident_string_dec n (sev env) with *)
+(*              | Some v' => (st, Rval [v']) *)
+(*              | None => (st, Rerr (Rabort Rtype_error)) *)
+(*              end *)
+(*   | ECon cn es' => if do_con_check (sec env) cn (length es') *)
+(*                   then match eval_or_match true (rev es') fuel st env uu uu with *)
+(*                        | (st', Rval vs) => *)
+(*                          match build_conv (sec env) cn (rev vs) with *)
+(*                          | Some v' => (st', Rval [v']) *)
+(*                          | None => (st', Rerr (Rabort Rtype_error)) *)
+(*                          end *)
+(*                        | res => res *)
+(*                        end *)
+(*                   else (st, Rerr (Rabort Rtype_error)) *)
+(*   | EFun x e => (st, Rval [Closure env x e]) *)
+(*   | EApp op es => match fuel with *)
+(*                  | 0 => (st, Rerr (Rabort Rtimeout_error)) *)
+(*                  | S fuel' => match eval_or_match true (rev es) fuel' st env uu uu with *)
+(*                           | (st', Rval vs) => if op_eq_dec op Opapp *)
+(*                                              then match do_opapp (rev vs) with *)
+(*                                                   | Some (env', e) => eval_or_match true [e] fuel' st' env' uu uu *)
+(*                                                   | None => (st', Rerr (Rabort Rtype_error)) *)
+(*                                                   end *)
+(*                                              else match do_app _ (refs st', ffi st') op (rev vs) with *)
+(*                                                   | Some ((refs, ffi), r) => ({| refs := refs; *)
+(*                                                                                 ffi  := ffi; *)
+(*                                                                                 clock := clock st'; *)
+(*                                                                                 next_type_stamp := next_type_stamp st' ; *)
+(*                                                                                 next_exn_stamp := next_exn_stamp st' *)
+(*                                                                              |}, *)
+(*                                                                              list_result r) *)
+(*                                                   | None => (st', Rerr (Rabort Rtype_error)) *)
+(*                                                   end *)
+(*                           | res => res *)
+(*                           end *)
+(*                  end *)
+(*   | EMat e pes => match eval_or_match true [e] fuel st env uu uu with *)
+(*                  | (st', Rval (v'::vs')) => *)
+(*                    eval_or_match false pes fuel st' env v' bind_exn_v *)
+
+(*                  | res => res *)
+(*                  end *)
+(*   | ELannot e l => eval_or_match true [e] fuel st env uu uu *)
+(*   end. *)
+(* Proof. *)
+(*   induction e; *)
+(*   intros; *)
+(*   simp eval_or_match; *)
+(*   try (reflexivity). *)
+(*   destruct fuel; simp eval_or_match; reflexivity. *)
+(* Qed. *)
+
+(* Lemma Forall''_image A B : forall (f : A -> B) l, *)
+(*   Forall'' (fun y => exists x, y = f x) l -> exists l', l = map f l'. *)
+(*   intros. *)
+(*   induction X. *)
+(*   exists []. reflexivity. *)
+(*   destruct p. *)
+(*   rewrite H; clear H. *)
+(*   destruct IHX. *)
+(*   exists (x0::x1). *)
+(*   simpl. *)
+(*   rewrite <- H. reflexivity. *)
+(* Qed. *)
+
+(* Lemma eval_sing_inc_fuel : forall (f : nat) (e : exp) (st st' : state A) *)
+(*                             (env : sem_env val) (res : result (list val) val), *)
+(*     res <> Rerr (Rabort Rtimeout_error) -> *)
+(*     evaluate [e] f st env = (st', res) -> *)
+(*     evaluate [e] (S f) st env = (st', res). *)
+(* Proof. *)
+(*   induction f. *)
+(*   intros. *)
+(*   unfold evaluate in *. *)
+(*   funelim (eval_or_match true [e] 0 st env uu uu). *)
+(*   apply H; try (assumption). *)
+(*   unfold eq_rect. *)
+(*   intros. simpl. rewrite H1. *)
+(*   Check eval_or_match_elim. *)
+(*   Check eq_rect. *)
+(* Check eval_or_match_elim. *)
+Check eq_refl.
+
+Axiom USOP : forall (U : Type) (x y:U) (p1 p2:x = y), p1 = p2.
+
+Lemma eval_or_match_inc_fuel_val : forall (f : nat) (sel : bool)
+                                     (es : if sel then list exp else list (pat * exp)) (st st' : state A)
+                                     (env : sem_env val) (match_v err_v : val) (vs : list val),
+    eval_or_match sel es f st env match_v err_v = (st', Rval vs) ->
+    eval_or_match sel es (S f) st env match_v err_v = (st', Rval vs).
+Proof.
+  intros.
+  funelim (eval_or_match sel es f st env match_v err_v).
+  - simp eval_or_match in *.
+  - simp eval_or_match in *.
+    break_if.
+    + destruct (eval_or_match true (rev l) fuel st env uu uu) eqn:eval1.
+      rewrite <- eval1 in H.
+      destruct r.
+      * apply H in eval1.
+        rewrite eval1.
+        break_match.
+        assumption.
+        inv Heqcall.
+        inv H0.
+      * inv Heqcall.
+        inv H0.
+    + inv Heqcall.
+      inv H0.
+  - simp eval_or_match. rewrite Heqcall. assumption.
+  - simp eval_or_match. rewrite Heqcall. assumption.
+  - rewrite <- Heqcall in H. inv H.
+  - simp eval_or_match in *.
+    destruct (eval_or_match true (rev l0) n st env uu uu) eqn:eval1.
+    destruct r.
+    * rewrite <- eval1 in H.
+      apply H in eval1.
+      rewrite eval1.
+      break_if.
+      + break_match.
+        -- break_let.
+           simpl in H0.
+           unfold eq_rect in Heqcall. simpl in *.
+           remember (@sigmaI Type (fun x => sigma (fun b : bool => sigma (fun l : if b then list exp else list (pat * exp) => sigma (fun n => sigma (fun st : state x => sigma (fun sem => sigma (fun v1 => val ))))))) A
+                 (@sigmaI bool (fun b : bool => sigma (fun l : if b then list exp else list (pat * exp) => sigma (fun n => sigma (fun st => sigma (fun sem => sigma (fun v1 => val )))))) true
+                          (@sigmaI (list exp) (fun l => sigma (fun n => sigma (fun st => sigma (fun sem => sigma (fun v1 => val ))))) [e0]
+                                   (@sigmaI nat (fun n => sigma (fun st => sigma (fun sem => sigma (fun v1 => val )))) n
+                                            (@sigmaI (state A) (fun st => sigma (fun sem => sigma (fun v1 => val ))) s
+                                                     (@sigmaI (sem_env val) (fun sem => sigma (fun v1 => val )) s0
+                                                              (@sigmaI val (fun v1 => val) uu uu)))))))
+             as ididit.
+           assert (ididit = ididit).
+           auto.
+           rewrite Heqididit in H2.
+
+           specialize (H0 s (Rval vs) vs e p s0 e0 n true [e0] s st' s0 uu uu vs H1 H2).
+           Check USOP.
+           assert (H2 = eq_refl).
+           apply USOP.
+           apply H0.
+           unfold eq_rect.
+           rewrite H3.
+           reflexivity.
+        -- inv H1.
+      + break_match. auto.
+        inv H1.
+    * inv H1.
+  - simp eval_or_match in *.
+    destruct (eval_or_match true [e0] fuel st env uu uu) eqn:eval1.
+    rewrite <- eval1 in H.
+    destruct r.
+    apply H in eval1.
+    rewrite eval1.
+    destruct l.
+    assumption.
+    remember (@sigmaI Type (fun x => sigma (fun b : bool => sigma (fun l : if b then list exp else list (pat * exp) => sigma (fun n => sigma (fun st : state x => sigma (fun sem => sigma (fun v1 => val ))))))) A
+                      (@sigmaI bool (fun b : bool => sigma (fun l : if b then list exp else list (pat * exp) => sigma (fun n => sigma (fun st => sigma (fun sem => sigma (fun v1 => val )))))) false
+                               (@sigmaI (list (pat * exp)) (fun l => sigma (fun n => sigma (fun st => sigma (fun sem => sigma (fun v1 => val ))))) l1
+                                        (@sigmaI nat (fun n => sigma (fun st => sigma (fun sem => sigma (fun v1 => val )))) fuel
+                                                 (@sigmaI (state A) (fun st => sigma (fun sem => sigma (fun v1 => val ))) s
+                                                          (@sigmaI (sem_env val) (fun sem => sigma (fun v1 => val )) env
+                                                                   (@sigmaI val (fun v1 => val) v bind_exn_v)))))))
+             as ididit.
+           assert (ididit = ididit).
+           auto.
+           rewrite Heqididit in H2.
+
+    specialize (H0 s (Rval vs) vs v vs fuel false l1 s st' env v bind_exn_v vs H1 H2).
+    clear Heqididit.
+    clear ididit.
+    apply H0.
+    unfold eq_rect.
+    assert (H2 = eq_refl).
+    apply USOP.
+    rewrite H3.
+    reflexivity.
+    inv H1.
+  - simp eval_or_match in *.
+  - simp eval_or_match in *.
+    destruct (eval_or_match true [e] fuel st env uu uu) eqn:eval1.
+    rewrite <- eval1 in H.
+    destruct r.
+    apply H in eval1.
+    rewrite eval1.
+    destruct (eval_or_match true (e0::l) fuel s env uu uu) eqn:eval2.
+    destruct r.
+    remember (@sigmaI Type (fun x => sigma (fun b : bool => sigma (fun l : if b then list exp else list (pat * exp) => sigma (fun n => sigma (fun st : state x => sigma (fun sem => sigma (fun v1 => val ))))))) A
+                      (@sigmaI bool (fun b : bool => sigma (fun l : if b then list exp else list (pat * exp) => sigma (fun n => sigma (fun st => sigma (fun sem => sigma (fun v1 => val )))))) true
+                               (@sigmaI (list exp) (fun l => sigma (fun n => sigma (fun st => sigma (fun sem => sigma (fun v1 => val ))))) (e0::l)
+                                        (@sigmaI nat (fun n => sigma (fun st => sigma (fun sem => sigma (fun v1 => val )))) fuel
+                                                 (@sigmaI (state A) (fun st => sigma (fun sem => sigma (fun v1 => val ))) s
+                                                          (@sigmaI (sem_env val) (fun sem => sigma (fun v1 => val )) env
+                                                                   (@sigmaI val (fun v1 => val) uu uu)))))))
+             as ididit.
+           assert (ididit = ididit).
+           auto.
+           rewrite Heqididit in H2.
+
+    specialize (H0 s (Rval vs) vs fuel true (e0::l) s s0 env uu uu l1 eval2 H2).
+    unfold eq_rect in H0.
+    assert (H2 = eq_refl).
+    apply USOP.
+    rewrite H3 in H0.
+    assert (eval_or_match true (e0 :: l) fuel s env uu uu =
+            eval_or_match true (e0 :: l) fuel s env uu uu) by congruence.
+    rewrite H0. assumption.
+    congruence.
+    inv H1.
+    inv H1.
+  - simp eval_or_match in *.
+  - simp eval_or_match in *.
+    clear Heqcall.
+    break_match.
+    break_match.
+    apply H.
+    assumption.
+    assumption.
+    inv H1.
+
+    remember (@sigmaI Type (fun x => sigma (fun b : bool => sigma (fun l : if b then list exp else list (pat * exp) => sigma (fun n => sigma (fun st : state x => sigma (fun sem => sigma (fun v1 => val ))))))) A
+                      (@sigmaI bool (fun b : bool => sigma (fun l : if b then list exp else list (pat * exp) => sigma (fun n => sigma (fun st => sigma (fun sem => sigma (fun v1 => val )))))) true
+                               (@sigmaI (list exp) (fun l => sigma (fun n => sigma (fun st => sigma (fun sem => sigma (fun v1 => val ))))) [e]
+                                        (@sigmaI nat (fun n => sigma (fun st => sigma (fun sem => sigma (fun v1 => val )))) fuel
+                                                 (@sigmaI (state A) (fun st => sigma (fun sem => sigma (fun v1 => val ))) st
+                                                          (@sigmaI (sem_env val) (fun sem => sigma (fun v1 => val )) {| sev := nsAppend (alist_to_ns a) (sev env); sec := sec env |}
+                                                                   (@sigmaI val (fun v1 => val) uu uu)))))))
+             as ididit.
+    assert (ididit = ididit).
+    auto.
+    rewrite Heqididit in H2.
+    unfold eq_rect.
+    assert (H2 = eq_refl).
+    apply USOP.
+    Check H0.
+    specialize (H0 n a fuel true [e] st st' {| sev := nsAppend (alist_to_ns a) (sev env); sec := sec env |} uu uu vs H1 H2).
+    apply H0.
+    unfold eq_rect.
+    rewrite H3.
+    congruence.
+    inv H1.
+Qed.
+
+Lemma eval_or_match_inc_fuel_res : forall (f : nat) (sel : bool)
+                                     (es : if sel then list exp else list (pat * exp)) (st st' : state A)
+                                     (env : sem_env val) (match_v err_v : val) (res : result (list val) val),
+    res <> Rerr (Rabort Rtimeout_error) ->
+    eval_or_match sel es f st env match_v err_v = (st', res) ->
+    eval_or_match sel es (S f) st env match_v err_v = (st', res).
+Proof.
+  intros.
+  funelim (eval_or_match sel es f st env match_v err_v).
+  - simp eval_or_match in *.
+  - simp eval_or_match in *.
+    clear Heqcall.
+    break_match.
+    destruct (eval_or_match true (rev l) fuel st env uu uu) eqn:eval1.
+    rewrite <- eval1 in H.
+    apply H in eval1.
+    rewrite eval1.
+    destruct r.
+    break_match; assumption.
+    inv H1.
+    congruence.
+    destruct r.
+    congruence.
+    congruence.
+    congruence.
+  - simp eval_or_match in *.
+  - simp eval_or_match in *.
+  - simp eval_or_match in *. congruence.
+  - simp eval_or_match in *.
+    destruct (eval_or_match true (rev l0) n st env uu uu) eqn:eval1.
+    rewrite <- eval1 in H.
+    apply H in eval1.
+    rewrite eval1.
+    break_match.
+    + break_if.
+      * break_match.
+        -- break_let.
+           simpl in H0.
+           remember (@sigmaI Type (fun x => sigma (fun b : bool => sigma (fun l : if b then list exp else list (pat * exp) => sigma (fun n => sigma (fun st : state x => sigma (fun sem => sigma (fun v1 => val ))))))) A
+                 (@sigmaI bool (fun b : bool => sigma (fun l : if b then list exp else list (pat * exp) => sigma (fun n => sigma (fun st => sigma (fun sem => sigma (fun v1 => val )))))) true
+                          (@sigmaI (list exp) (fun l => sigma (fun n => sigma (fun st => sigma (fun sem => sigma (fun v1 => val ))))) [e0]
+                                   (@sigmaI nat (fun n => sigma (fun st => sigma (fun sem => sigma (fun v1 => val )))) n
+                                            (@sigmaI (state A) (fun st => sigma (fun sem => sigma (fun v1 => val ))) s
+                                                     (@sigmaI (sem_env val) (fun sem => sigma (fun v1 => val )) s0
+                                                              (@sigmaI val (fun v1 => val) uu uu)))))))
+             as ididit.
+           assert (ididit = ididit).
+           auto.
+           rewrite Heqididit in H3.
+
+           Check H0.
+           specialize (H0 s res l e p s0 e0 n true [e0] s st' s0 uu uu res H1 H2 H3).
+           Check USOP.
+           assert (H3 = eq_refl).
+           apply USOP.
+           apply H0.
+           unfold eq_rect.
+           rewrite H4.
+           reflexivity.
+        -- congruence.
+      * break_match; auto.
+    + congruence.
+    + destruct r; congruence.
+  - simp eval_or_match in *.
+    destruct (eval_or_match true [e0] fuel st env uu uu) eqn:eval1.
+    rewrite <- eval1 in H.
+    apply H in eval1.
+    rewrite eval1.
+    destruct r; auto.
+    destruct l; auto.
+    remember (@sigmaI Type (fun x => sigma (fun b : bool => sigma (fun l : if b then list exp else list (pat * exp) => sigma (fun n => sigma (fun st : state x => sigma (fun sem => sigma (fun v1 => val ))))))) A
+                      (@sigmaI bool (fun b : bool => sigma (fun l : if b then list exp else list (pat * exp) => sigma (fun n => sigma (fun st => sigma (fun sem => sigma (fun v1 => val )))))) false
+                               (@sigmaI (list (pat * exp)) (fun l => sigma (fun n => sigma (fun st => sigma (fun sem => sigma (fun v1 => val ))))) l1
+                                        (@sigmaI nat (fun n => sigma (fun st => sigma (fun sem => sigma (fun v1 => val )))) fuel
+                                                 (@sigmaI (state A) (fun st => sigma (fun sem => sigma (fun v1 => val ))) s
+                                                          (@sigmaI (sem_env val) (fun sem => sigma (fun v1 => val )) env
+                                                                   (@sigmaI val (fun v1 => val) v bind_exn_v)))))))
+             as ididit.
+    assert (ididit = ididit).
+    auto.
+    rewrite Heqididit in H3.
+    Check H0.
+    specialize (H0 s res l v l fuel false l1 s st' env v bind_exn_v res H1 H2 H3).
+    apply H0.
+    unfold eq_rect.
+    assert (H3 = eq_refl).
+    apply USOP.
+    rewrite H4.
+    reflexivity.
+    destruct r; congruence.
+  - simp eval_or_match in *.
+  - simp eval_or_match in *.
+    clear Heqcall.
+    destruct (eval_or_match true [e] fuel st env uu uu) eqn:eval1.
+    rewrite <- eval1 in H.
+    apply H in eval1.
+    rewrite eval1.
+    remember (@sigmaI Type (fun x => sigma (fun b : bool => sigma (fun l : if b then list exp else list (pat * exp) => sigma (fun n => sigma (fun st : state x => sigma (fun sem => sigma (fun v1 => val ))))))) A
+                      (@sigmaI bool (fun b : bool => sigma (fun l : if b then list exp else list (pat * exp) => sigma (fun n => sigma (fun st => sigma (fun sem => sigma (fun v1 => val )))))) true
+                               (@sigmaI (list exp) (fun l => sigma (fun n => sigma (fun st => sigma (fun sem => sigma (fun v1 => val ))))) (e0::l)
+                                        (@sigmaI nat (fun n => sigma (fun st => sigma (fun sem => sigma (fun v1 => val )))) fuel
+                                                 (@sigmaI (state A) (fun st => sigma (fun sem => sigma (fun v1 => val ))) s
+                                                          (@sigmaI (sem_env val) (fun sem => sigma (fun v1 => val )) env
+                                                                   (@sigmaI val (fun v1 => val) uu uu)))))))
+      as ididit.
+    assert (ididit = ididit) by auto.
+    rewrite Heqididit in H3.
+    destruct r.
+    + destruct (eval_or_match true (e0::l) fuel s env uu uu) eqn:eval2.
+      destruct r.
+      * destruct l0.
+        -- assert (HneqValErr : ((Rval l1 : result (list val) val) <> Rerr (Rabort Rtimeout_error))) by congruence.
+        specialize (H0 s (Rval l1) l1 fuel true (e0::l) s s0 env uu uu (Rval l1) HneqValErr eval2 H3).
+        unfold eq_rect in H0.
+        assert (H3 = eq_refl) by apply USOP.
+        rewrite H4 in H0.
+        rewrite H0; congruence.
+        -- assert (HneqValErr : ((Rval l1 : result (list val) val) <> Rerr (Rabort Rtimeout_error))) by congruence.
+           specialize (H0 s (Rval (l1)) l1 fuel true (e0::l) s s0 env uu uu (Rval (l1)) HneqValErr eval2 H3).
+           unfold eq_rect in H0.
+           assert (H3 = eq_refl) by apply USOP.
+           rewrite H4 in H0.
+           rewrite H0; congruence.
+        * inv H2.
+          specialize (H0 s (Rerr e1) l0 fuel true (e0::l) s st' env uu uu (Rerr e1) H1 eval2 H3).
+          unfold eq_rect in H0.
+          assert (H3 = eq_refl) by apply USOP.
+          rewrite H2 in H0.
+          rewrite H0; congruence.
+    + congruence.
+    + destruct r; congruence.
+  - simp eval_or_match in *.
+  - simp eval_or_match in *.
+    break_if.
+    + break_match.
+      * apply H; assumption.
+      * congruence.
+      * remember (@sigmaI Type (fun x => sigma (fun b : bool => sigma (fun l : if b then list exp else list (pat * exp) => sigma (fun n => sigma (fun st : state x => sigma (fun sem => sigma (fun v1 => val ))))))) A
+                          (@sigmaI bool (fun b : bool => sigma (fun l : if b then list exp else list (pat * exp) => sigma (fun n => sigma (fun st => sigma (fun sem => sigma (fun v1 => val )))))) true
+                                   (@sigmaI (list exp) (fun l => sigma (fun n => sigma (fun st => sigma (fun sem => sigma (fun v1 => val ))))) [e]
+                                            (@sigmaI nat (fun n => sigma (fun st => sigma (fun sem => sigma (fun v1 => val )))) fuel
+                                                     (@sigmaI (state A) (fun st => sigma (fun sem => sigma (fun v1 => val ))) st
+                                                              (@sigmaI (sem_env val) (fun sem => sigma (fun v1 => val )) {| sev := (nsAppend (alist_to_ns a) (sev env)); sec := sec env |}
+                                                                       (@sigmaI val (fun v1 => val) uu uu)))))))
+          as ididit.
+        assert (ididit = ididit) by auto.
+        rewrite Heqididit in H3.
+        Check H0.
+        specialize (H0 n a fuel true [e] st st' {| sev := nsAppend
+                                                            (alist_to_ns a)
+                                                            (sev env);
+                                                   sec := sec env |}
+                       uu uu res H1 H2 H3).
+        apply H0.
+        unfold eq_rect.
+        assert (H3 = eq_refl) by apply USOP.
+        rewrite H4.
+        congruence.
+    + congruence.
+Qed.
+
+
+Lemma evaluate_inc_fuel_res : forall (f : nat) (es : list exp) (st st' : state A)
+                                (env : sem_env val) (res : result (list val) val),
+    res <> Rerr (Rabort Rtimeout_error) ->
+    evaluate es f st env = (st', res) ->
+    evaluate es (S f) st env = (st', res).
+Proof.
+  intros.
+  apply eval_or_match_inc_fuel_res; assumption.
+Qed.
+
+Lemma more_fuel_same_result : forall (f f' : nat) (st st' : state A) (env : sem_env val) (res : result (list val) val) (es : list exp),
+    f <= f' ->
+    res <> Rerr (Rabort Rtimeout_error) ->
+    evaluate es f st env = (st', res) ->
+    evaluate es f' st env = (st', res).
+Proof.
+  intros f f'. generalize dependent f.
+  induction f';
+    intros f st st' env res es H H1 contra;
+    inv H; auto.
+    apply eval_or_match_inc_fuel_res; auto.
+    apply IHf' with f; auto.
+Qed.
+
+Theorem ELannot_does_nothing : forall (e : exp) (l : locs) (f : nat) (st : state A) (env : sem_env val),
+    evaluate [ELannot e l] f st env = evaluate [e] f st env.
+Proof.
+  intros e l f st env.
+  unfold evaluate.
+  simp eval_or_match.
+  congruence.
+Qed.
+
+Ltac more_fuel_same_result_quick :=
+  match goal with
+  | [ H0 : evaluate ?es ?f ?st ?env = (?st',?res), H1 : context[evaluate ?es ?f' ?st ?env] |- _ ] =>
+    let H := fresh "H" in
+    let Hass := fresh "Hass" in
+    let Hass0 := fresh "Hass0" in
+    assert (H : evaluate es f st env = (st',res)) by apply H0;
+    assert (Hass : f <= f') by omega;
+    assert (Hass0 : res <> (Rerr (Rabort Rtimeout_error))) by (simpl; congruence);
+    apply (more_fuel_same_result f f' st st' env res es Hass Hass0) in H;
+    rewrite H in H1;
+    clear Hass Hass0 H
+  end.
+
+Ltac match_exp_same :=
+  match goal with
+  | [H : context[ match ?x with
+                  | ECon _ _ => ?y
+                  | EVar _   => ?y
+                  | EFun _ _ => ?y
+                  | EApp _ _ => ?y
+                  | EMat _ _ => ?y
+                  | ELannot _ _ => ?y
+                  end] |- _ ] =>
+    let Hass := fresh "Hass" in
+    assert (Hass : match x with
+                   | ECon _ _ => y
+                   | EVar _   => y
+                   | EFun _ _ => y
+                   | EApp _ _ => y
+                   | EMat _ _ => y
+                   | ELannot _ _ => y
+                   end
+                   = y) by (destruct x; reflexivity);
+    rewrite Hass in H; clear Hass
+  end.
+
+
+Theorem plus_vs_cake_plus : forall (m n t f : nat) (m_exp n_exp : exp) (m_val n_val m_n_val : val) (env : sem_env val),
+    environment_extended my_env env ->
+    evaluate [m_exp] f my_st my_env = (my_st, Rval [m_val]) ->
+    evaluate [n_exp] f my_st my_env = (my_st, Rval [n_val]) ->
+    nat_rel_cake_nat t m m_val ->
+    nat_rel_cake_nat t n n_val ->
+    evaluate [(EApp (Opapp) ((EApp (Opapp) ((EVar (Short ("plus"%string)))::m_exp::nil))::n_exp::nil))]
+             f my_st my_env =
+    (my_st, Rval [m_n_val]) ->
+    nat_rel_cake_nat t (m+n) m_n_val.
+Proof.
+  intros.
+  unfold evaluate in *.
+  apply eval_or_match_inc_fuel_res in H4; try congruence.
+  apply eval_or_match_inc_fuel_res in H4; try congruence.
+  simp eval_or_match in *; simpl in *.
+  rewrite eval_or_match_cons in H4; simpl in *.
+  apply eval_or_match_inc_fuel_res in H1; try congruence.
+  rewrite H1 in H4.
+  simp eval_or_match in *; simpl in *.
+  simp eval_or_match in *; simpl in *.
+  rewrite H0 in H4.
+  simp eval_or_match in *; simpl in *.
+  break_if; try congruence.
+  simp eval_or_match in *; simpl in *.
+  simp eval_or_match in *; simpl in *.
+  simp eval_or_match in *; simpl in *.
+  break_match
+
+
+
+  intros.
+  revert H H0 H1 H3 H4. revert env m_n_val n_val n_exp m_exp f n.
+  induction H2; unfold evaluate in *.
+  - intros.
+    apply eval_or_match_inc_fuel_res in H4; try congruence.
+    apply eval_or_match_inc_fuel_res in H4; try congruence.
+    apply eval_or_match_inc_fuel_res in H4; try congruence.
+    simp eval_or_match in H4.
+    simpl in*.
+    simp eval_or_match in H4.
+    apply eval_or_match_inc_fuel_res in H1; try congruence.
+    apply eval_or_match_inc_fuel_res in H1; try congruence.
+    rewrite H1 in H4.
+    simp eval_or_match in H4.
+    simpl in *.
+    simp eval_or_match in H4.
+    apply eval_or_match_inc_fuel_res in H0; try congruence.
+    rewrite H0 in H4.
+    simp eval_or_match in H4.
+    simpl in *.
+    simp eval_or_match in H4.
+    simpl in *.
+    destruct (op_eq_dec); try congruence.
+    simpl in *.
+    simp eval_or_match in H4.
+    simpl in *.
+    simp eval_or_match in H4.
+    destruct NoDuplicates_dec; try congruence.
+    simpl in *.
+    break_if; try congruence.
+    simp eval_or_match in H4.
+    simpl in *.
+    inv H4.
+    assumption.
+  - intros.
+    apply eval_or_match_inc_fuel_res in H4; try congruence.
+    apply eval_or_match_inc_fuel_res in H4; try congruence.
+    apply eval_or_match_inc_fuel_res in H4; try congruence.
+    simp eval_or_match in H4; simpl in *.
+    simp eval_or_match in H4; simpl in *.
+    apply eval_or_match_inc_fuel_res in H1; try congruence.
+    apply eval_or_match_inc_fuel_res in H1; try congruence.
+    rewrite H1 in H4.
+    simp eval_or_match in H4; simpl in *.
+    simp eval_or_match in H4; simpl in *.
+    apply eval_or_match_inc_fuel_res in H0; try congruence.
+    rewrite H0 in H4.
+    simp eval_or_match in H4; simpl in *.
+    break_if; try congruence.
+    simp eval_or_match in H4; simpl in *.
+    simp eval_or_match in H4; simpl in *.
+    simp eval_or_match in H4.
+    Opaque NoDuplicates_dec.
+    destruct NoDuplicates_dec.
+    simpl in H4.
+    break_if. break_if; try congruence.
+    clear Heqs.
+    simp eval_or_match in H4; simpl in *.
+    simp eval_or_match in H4; simpl in *.
+    simp eval_or_match in H4; simpl in *.
+    simp eval_or_match in H4; simpl in *.
+    simp eval_or_match in H4; simpl in *.
+    simp eval_or_match in H4; simpl in *.
+    assert (SECCLEAN : forall (V : Type) (e : sem_env V) x, sec (update_sev e x) = sec e) by reflexivity.
+    simp eval_or_match in H4; simpl in *.
+    break_if; try congruence.
+    break_if; try congruence.
+    simp eval_or_match in H4; simpl in *.
+    simp eval_or_match in H4; simpl in *.
+    simp eval_or_match in H4. rewrite SECCLEAN in H4.
